tightened framing invariants in Handshake.fsti; the basic structure of frame_epoch lemma goes through, but there is still one admit remaining there

src/tls/StatefulLHAE.fsti
@@ -1,10 +1,6 @@
 module StatefulLHAE
-
 // Stateful, agile, length-hiding authenticated encryption with additional data
 // (implemented by appending a fragment sequence number to the additional data)
-
-// this interface separates the TLS machinery from its authenticated-encryption schemes
-// it also experiments with predicate abstraction (not so clear with heap accesses)
 
 open FStar.Heap
 open FStar.HyperHeap
@@ -16,183 +12,167 @@ open Platform.Bytes
 open TLSError
 open TLSInfo
 open Range
+open LHAEPlain
+open AEAD_GCM
 open StatefulPlain
 
 type id = AEAD_GCM.gid //TODO: TEMPORARY, until we add back LHAE 
 
+let snoc = Content.snoc //why can't it go in the library!?
+//type cipher = StatefulPlain.cipher
+//TODO: this is a workaround for #383 in F* (eta expansion needed for type abbreviations)
 type cipher (i:id) = StatefulPlain.cipher i
-let snoc = Content.snoc // why can't it go in the library!?
 
 (* decrypted plaintexts, within a range computed from the cipher length *)
 type dplain (i:id) (ad:adata i) (c:cipher i) =
-    plain i ad (Range.cipherRangeClass i (length c))
+  StatefulPlain.plain i ad (cipherRangeClass i (length c))
 
 type entry (i:id) = (* records that c is an encryption of p with ad *)
-  | Entry: c: cipher i -> ad:adata i -> p:dplain i ad c -> entry i
+  | Entry: c:cipher i -> ad:adata i -> p:dplain i ad c -> entry i
 
-// relocate?
 type is_seqn (n:nat) = repr_bytes n <= 8
-type seqn = n:nat { repr_bytes n <= 8 }
+type seqn_t = n:nat { repr_bytes n <= 8 } 
 
 (* typing the log that specifies StatefulLHAE *)
 type st_log_t (r:rid) (i:id) = rref r (s:seq (entry i))
 
-(* CF we might merge those types into State id role *)
-type writer (i:id)
-val writer_region : #i:id -> writer i   -> Tot rid
-val writer_log    : #i:id -> w:writer i -> Tot (st_log_t (writer_region w) i)
-val writer_seqn   : #i:id -> w:writer i -> Tot (rref (writer_region w) seqn)
-
-type reader (i:id)
-val reader_region : #i:id -> reader i   -> Tot rid
-val reader_log    : #i:id -> r:reader i -> Tot (st_log_t (reader_region r) i)
-val reader_seqn   : #i:id -> r:reader i -> Tot (rref (reader_region r) seqn)
-
-opaque type matching (#i:id) (r:reader i) (w:writer i)
-
-val public_matching: #i:id -> r:reader i -> w:writer i ->
-  Lemma ( matching r w ==> (
-            reader_region r = writer_region w
-         /\ reader_log r    = writer_log w
-         /\ reader_seqn r  <> writer_seqn w ))
-
-type both (i:id) = rw:(reader i * writer i){matching (fst rw) (snd rw)}
-
-opaque type st_inv (#i:id) (d:reader i) (e:writer i) (h:HyperHeap.t)
-
-val public_st_inv: #i:id -> d:reader i -> e:writer i -> h:HyperHeap.t ->
-  Lemma ( st_inv d e h ==> (
-       matching d e
-    /\ Map.contains h (reader_region d)
-    /\ Let (sel h (writer_log e)) (fun st ->
-       Let (sel h (reader_seqn d)) (fun r ->
-       Let (sel h (writer_seqn e)) (fun w ->
-         w = Seq.length st /\ r <= w )))))
-
-
-val gen: r0:rid -> i:id ->
-         ST (both i)
-            (requires (fun h -> True))
-            (ensures (fun h0 (rw:both i) h1 ->
-                 modifies Set.empty h0 h1
-              /\ fresh_region (reader_region (fst rw)) h0 h1
-              /\ extends (reader_region (fst rw)) r0
-              /\ st_inv (fst rw) (snd rw) h1
-              /\ sel h1 (writer_log (snd rw)) = Seq.createEmpty
-              /\ sel h1 (reader_seqn (fst rw)) = 0
-              ))
-
-val leak_reader: i:id{~(safeId i)} -> reader i ->
-                 ST (bytes)
-                    (requires (fun h -> True))
-                    (ensures (fun h0 s h1 ->
-                         modifies Set.empty h0 h1 ))
-
-val leak_writer: i:id{~(safeId i)} -> writer i ->
-                 ST (bytes)
-                    (requires (fun h -> True))
-                    (ensures (fun h0 s h1 ->
-                         modifies Set.empty h0 h1 ))
-
-(*
-val coerce_reader: r0:rid -> i:id{~(safeId i)} -> kv:key i -> iv: iv i->
-                   ST (reader i)
-                      (requires (fun h -> True))
-                      (ensures (fun h0 s h1 ->
-                           modifies Set.empty h0 h1
-                          /\ extends (reader_region s) r0
-                          /\ fresh_region (State.region (reader_key s)) h0 h1
-                          /\ sel h1 (reader_log s) = Seq.createEmpty
-                          /\ sel h1 (reader_seqn s) = 0))
-
-val coerce_writer: r0:rid -> i:id{~(safeId i)} -> kv:key i -> iv: iv i->
-                     ST (writer i)
-                        (requires (fun h -> True))
-                        (ensures (fun h0 s h1 ->
-                             modifies Set.empty h0 h1
-                            /\ extends (writer_region s) r0
-                            /\ fresh_region (State.region (writer_key s)) h0 h1
-                            /\ sel h1 (writer_log s) = Seq.createEmpty
-                            /\ sel h1 (writer_seqn s) = 0))
-*)
-opaque type st_enc_inv (#i:id) (e:writer i) (h:HyperHeap.t) = exists (d:reader i). st_inv d e h
-
-val public_st_enc_inv: #i:id -> e:writer i -> h:HyperHeap.t ->
-  Lemma ( st_enc_inv e h ==> (
-       Let (sel h (writer_log e)) (fun st ->
-       Let (sel h (writer_seqn e)) (fun w ->
-         w == Seq.length st ))))
-
-let refs_in_e (#i:id) (e:writer i) = !{ as_ref (writer_log e), as_ref (writer_seqn e) }
-
-// let widen #i #ad r0 (r1:_ { Wider r1 r0 }) (f:plain i ad r0) : plain i ad r1 = f 
-let widen #i #ad #rg (c:cipher i) (f:plain i ad rg { Wider (Range.cipherRangeClass i (length c)) rg}) : dplain i ad c = 
-//  admit();
-  f
+(* typing the private log that specifies LHAE's implementation of StLHAE *)
+type gcm_log_t (r:rid) (i:gid) = rref r (s:seq (AEAD_GCM.entry i))
  
+type state (i:gid) (rw:rw) 
+type reader i = state i Reader
+type writer i = state i Writer
+val region        : #i:id -> #rw:rw -> state i rw -> Tot rid
+val peer_region   : #i:id -> #rw:rw -> state i rw -> Tot rid
+let log_region    = fun (#i:id) (#rw:rw) (s:state i rw) -> if rw=Reader then peer_region s else region s
+val log           : #i:id -> #rw:rw -> s:state i rw -> Tot (st_log_t (log_region s) i)
+val seqn          : #i:id -> #rw:rw -> s:state i rw -> Tot (rref (region s) seqn_t)
 
-val encrypt:
-  #i:id -> #ad:adata i -> #rg:range
-  -> wr:writer i
-  -> f:plain i ad rg
-  -> ST (cipher i)
-     (requires (fun h -> st_enc_inv wr h))
-//FIXME     (requires (fun h -> st_enc_inv wr h /\ is_seqn (sel h (writer_seqn wr) + 1)))
-     (ensures (fun h0 (c:cipher i) h1 ->
-                    st_enc_inv wr h1
-                /\  HyperHeap.modifies (Set.singleton (writer_region wr)) h0 h1
-                /\  Heap.modifies (refs_in_e wr) (Map.sel h0 (writer_region wr))
-                                                 (Map.sel h1 (writer_region wr))
-                /\  sel h1 (writer_seqn wr) = sel h0 (writer_seqn wr) + 1
-                /\  Wider  (Range.cipherRangeClass i (length c)) rg
-                /\  sel h1 (writer_log wr)  = snoc (sel h0 (writer_log wr)) (Entry c ad f)))
+opaque type matching (#i:gid) (r:reader i) (w:writer i)
 
+val unfold_matching: #i:id -> r:reader i -> w:writer i ->
+  Lemma ( matching r w ==> (
+            region r = peer_region w
+          /\ region w = peer_region r
+          /\ disjoint (region r) (region w)
+          /\ log r = log w))
 
-(* // should be provable from st_enc_inv's footprint *)
-(* val frame_encrypt: #i:id -> wr:writer i -> h0:_ -> h1:_ -> *)
-(*   Lemma (requires st_enc_inv wr h0 /\  *)
-(*                   Map.Equal (restrict (Set.singleton (writer_region wr)) h0) *)
-(*                             (restrict (Set.singleton (writer_region wr)) h1)) *)
-(*         (ensures st_enc_inv wr h1) *)
+type both (i:gid) = rw:(reader i * writer i){matching (fst rw) (snd rw)}
 
-opaque type st_dec_inv (#i:id) (d:reader i) (h:HyperHeap.t) = exists (e:writer i). st_inv d e h
+opaque type st_inv (#i:gid) (r:reader i) (w:writer i) (h:HyperHeap.t) 
 
-(* val frame_decrypt: #i:id -> rd:reader i -> h0:_ -> h1:_ -> *)
-(*   Lemma (requires st_dec_inv rd h0 /\  *)
-(*                   Map.Equal (restrict (Set.singleton (reader_region rd)) h0) *)
-(*                             (restrict (Set.singleton (reader_region rd)) h1)) *)
-(*         (ensures st_dec_inv rd h1) *)
+val unfold_st_inv: #i:id -> r:reader i -> w:writer i -> h:HyperHeap.t ->
+  Lemma ( st_inv r w h ==> (
+       matching r w
+    /\ Map.contains h (region r)  
+    /\ Map.contains h (region w)
+    /\ (let log = sel h (log w) in
+       let rctr = sel h (seqn r) in 
+       let wctr = sel h (seqn w) in 
+       wctr = Seq.length log
+       /\ rctr <= wctr )))
 
+let regions_of (#i:id) (#rw:rw) (s:state i rw) = 
+    Set.union (Set.singleton (region s))
+              (Set.singleton (peer_region s))
 
-//type Let (#a:Type) (=x:a) (body:(y:a{y=x}) -> Type) = body x
+let refs_in_w (#i:gid) (e:writer i) =
+  !{ as_ref (log e), as_ref (seqn e) }
 
-val decrypt:
-   #i:id
-   -> #ad:adata i
-   -> rd:reader i
-   -> c:cipher i //should be embedded in cipher i : {((length c) > (TLSConstants.aeadTagSize (alg i)))}
-   -> ST (option (dplain i ad c))
-         (requires (fun h ->
-              (safeId i ==> st_dec_inv rd h)
-           /\ is_seqn (sel h (reader_seqn rd) + 1)))
-         (ensures (fun h0 (res:option (dplain i ad c)) h1 -> True
-(* TODO
-                 HyperHeap.modifies (Set.singleton (reader_region rd)) h0 h1
-              /\ Heap.modifies !{as_ref (reader_seqn rd)} (Map.sel h0 (reader_region rd))
-                                                          (Map.sel h1 (reader_region rd))
-              /\ is_seqn (sel h0 (reader_seqn rd) + 1)
-              /\ Heap.contains (Map.sel h0 (reader_region rd)) (as_ref (reader_log rd))
-              /\ Let (sel h0 (reader_log rd))  (fun (log:seq (entry i){log=sel h0 (reader_log rd)}) ->
-                 Let (sel h0 (reader_seqn rd)) (fun (rctr:nat{rctr=sel h0 (reader_seqn rd)}) ->
-                   (safeId i
-                    ==>
-                      st_dec_inv rd h0
-                      /\ st_dec_inv rd h1
-                      /\  (if is_Some res
-                           then (sel h1 (reader_seqn rd) = rctr + 1
-                                /\ Some.v res == Entry.p (Seq.index log rctr))
-                           else ((Seq.length log=rctr                              // no more ciphers
-                                  \/ c <> Entry.c (Seq.index log rctr)             // wrong cipher
-                                  \/ ad =!= Entry.ad (Seq.index log rctr)))))))
-*)
-))  // wrong ad
+val frame_st_inv: #i:id -> r:reader i -> w:writer i ->  h0:_ -> h1:_ ->
+  Lemma (requires st_inv r w h0
+                  /\ equal_on (regions_of w) h0 h1)
+        (ensures st_inv r w h1)
+
+val gen: reader_parent:rid -> writer_parent:rid -> i:gid -> ST (both i)
+  (requires (fun h -> disjoint reader_parent writer_parent))
+  (ensures  (fun h0 (rw:both i) h1 ->
+      modifies Set.empty h0 h1
+    /\ (let r = fst rw in
+       let w = snd rw in
+      fresh_region (region r) h0 h1
+    /\ fresh_region (region w) h0 h1
+    /\ extends (region r) reader_parent
+    /\ extends (region w) writer_parent
+    /\ st_inv r w h1
+    /\ sel h1 (log w) = Seq.createEmpty
+    /\ sel h1 (seqn r) = 0)))
+    
+val leak_reader: i:gid{~(safeId i)} -> reader i -> ST bytes
+  (requires (fun h -> True))
+  (ensures  (fun h0 s h1 -> modifies Set.empty h0 h1 ))
+
+val leak_writer: i:gid{~(safeId i)} -> writer i -> ST bytes
+  (requires (fun h -> True))
+  (ensures  (fun h0 s h1 -> modifies Set.empty h0 h1 ))
+
+val coerce: r0:rid -> p0:rid {disjoint r0 p0} -> role:rw -> i:gid{~(safeId i)} -> kv:key i -> iv:iv i
+  -> ST (state i role)
+        (requires (fun h -> True))
+        (ensures  (fun h0 s h1 ->
+          modifies Set.empty h0 h1
+          /\ extends (region s) r0
+          /\ extends (peer_region s) p0
+          /\ fresh_region (region s) h0 h1
+          /\ fresh_region (peer_region s) h0 h1
+          /\ sel h1 (log s) = Seq.createEmpty
+          /\ sel h1 (seqn s) = 0))
+
+opaque type st_enc_inv (#i:gid) (w:writer i) (h:HyperHeap.t) =
+  exists (r:reader i).{:pattern (matching r w)} st_inv r w h
+
+val frame_st_enc_inv: #i:id -> w:writer i ->  h0:_ -> h1:_ ->
+  Lemma (requires st_enc_inv w h0
+                  /\ equal_on (regions_of w) h0 h1)
+        (ensures st_enc_inv w h1)
+
+val encrypt: #i:gid -> #ad:adata i
+  -> #rg:range{fst rg = snd rg /\ snd rg <= max_TLSPlaintext_fragment_length}
+  -> wr:writer i -> f:plain i ad rg -> ST (cipher i)
+  (requires (fun h -> st_enc_inv wr h /\ is_seqn (sel h (seqn wr) + 1)))
+  (ensures  (fun h0 (c:cipher i) h1 ->
+                  st_enc_inv wr h1
+                /\ modifies (Set.singleton (region wr)) h0 h1
+                /\ modifies_rref (region wr) (refs_in_w wr) h0 h1
+                /\ sel h1 (seqn wr) = sel h0 (seqn wr) + 1
+                /\ Wider (Range.cipherRangeClass i (length c)) rg
+                /\ sel h1 (log wr) = snoc (sel h0 (log wr)) (Entry c ad f)))
+
+opaque type st_dec_inv (#i:gid) (r:reader i) (h:HyperHeap.t) =
+  exists (w:writer i).{:pattern (matching r w)} st_inv r w h
+
+val frame_decrypt: #i:id -> rd:reader i -> h0:_ -> h1:_ ->
+  Lemma (requires (st_dec_inv rd h0 /\ 
+                   equal_on (regions_of rd) h0 h1))
+        (ensures st_dec_inv rd h1)
+ 
+(* (\* TODO: Replace Let in prims.fst with this definition? *\) *)
+type Let (#a:Type) (=x:a) (body:(y:a{y=x}) -> Type) = body x
+
+val decrypt: #i:gid -> #ad:adata i -> rd:reader i 
+  -> c:cipher i{length c > CoreCrypto.aeadTagSize (alg i)} 
+  -> ST (option (dplain i ad c))
+  (requires (fun h ->
+             (authId i ==> st_dec_inv rd h)
+           /\ is_seqn (sel h (seqn rd) + 1)))
+  (ensures (fun h0 (res:option (dplain i ad c)) h1 ->
+               modifies (Set.singleton (region rd)) h0 h1
+             /\ modifies_rref (region rd) !{as_ref (seqn rd)} h0 h1
+             /\ is_seqn (sel h0 (seqn rd) + 1)
+             /\ contains_ref (log rd) h0
+             /\ (Let (sel h0 (log rd))  (fun (lg:seq (entry i){lg=sel h0 (log rd)}) -> 
+                Let (sel h0 (seqn rd)) (fun (rctr:nat{rctr=sel h0 (seqn rd)}) ->
+               authId i
+               ==> st_dec_inv rd h0
+                /\ st_dec_inv rd h1
+                /\ rctr < Seq.length lg
+                /\ (if is_Some res
+                   then
+                    (sel h1 (seqn rd) = rctr + 1
+                     /\ Some.v res == Entry.p (Seq.index lg rctr))
+                   else
+                      Seq.length lg = rctr                 // no more ciphers
+                    \/ c <> Entry.c (Seq.index lg rctr)      // wrong cipher
+                    \/ ad =!= Entry.ad (Seq.index lg rctr)) // wrong ad
+             ))
+    )))
